src/PlutusIR/Transform/DeadCode2.v
@@ -23,6 +23,10 @@ Definition ftv : Term -> list string := Term.ftv.
 Definition disjoint {A} (xs ys : list A) : Prop :=
   Forall (fun v => ~ In v ys) xs.
 
+Definition unused_in (b : Binding) (t : Term) : Prop :=
+  disjoint (bvb b) (fv t) /\
+  disjoint (btvb b) (ftv t)
+.
 
 Inductive dc : Term -> Term -> Prop :=
   | dc_compat
@@ -30,31 +34,26 @@ Inductive dc : Term -> Term -> Prop :=
       (H_compat : Compat dc t t')
       : dc t t'
 
-      (* Note: This includes a case for Let, which are already covered by the following
-         four constructors. If we change this, there should be `compat` constructors for each of the
-         other AST constructor *)
-
+    (* Note: This compat case includes a case for Let, which are already
+    covered by the following four constructors (e.g. there is more than one way
+    to prove compatibility with let). If we change this, there should be `compat`
+    constructors for each of the other AST constructor *)
 
   | dc_delete_binding
       b bs t t'
-
-      (* Syntactic approximation of a pure binding *)
-      (H_pure : pure_binding [] b)
-
-      (* Its bound variables do not occur free in the post-term *)
-      (H_disjoint : disjoint (bvb b) (fv t'))
-      (H_disjoint_ty : disjoint (btvb b) (ftv t'))
-
-      (H_dc_bs : dc (Let NonRec       bs  t) t')
+      (H_pure : pure_binding [] b)          (* Syntactic approximation of a pure (terminating) binding *)
+      (H_unused : unused_in b t')           (* its bound variables do not occur free in the post-term *)
+      (H_dc_bs : dc (Let NonRec bs  t) t')
       : dc (Let NonRec (b :: bs) t) t'
 
   | dc_keep_binding
       b b' bs bs' t t'
-      (H_dc_t : dc t t')
       (H_dc_b : Compat_Binding dc b b')
-      (H_dc_bs : dc (Let NonRec       bs  t) (Let NonRec        bs'  t'))
+      (H_dc_bs : dc (Let NonRec bs t) (Let NonRec bs'  t'))
       : dc (Let NonRec (b :: bs) t) (Let NonRec (b' :: bs') t')
 
+
+  (* This rule allows for deleting the whole binding group *)
   | dc_delete_let_nil
       t t'
       (H_dc_t : dc t t')
@@ -63,9 +62,48 @@ Inductive dc : Term -> Term -> Prop :=
   | dc_compat_let_nil_nil
       t t'
       (H_dc_t : dc t t')
-      : dc (Let NonRec [] t) (Let NonRec [] t').
+      : dc (Let NonRec [] t) (Let NonRec [] t')
 
-  (* TODO: support Let Rec (See #42) *)
+  | dc_letrec
+      bs bs' t t'
+      (H_dc_rec : dc_rec bs' (Let Rec bs t) (Let Rec bs' t'))
+      : dc (Let Rec bs t) (Let Rec bs' t')
+
+with dc_rec : list Binding -> Term -> Term -> Prop :=
+
+  (*
+  Note: dc_rec does not include the possibility for the whole group to be
+  removed like for NonRec in dc.
+
+  This is because a rule like dc_rec_delete_binding needs to check if the bound
+  variables are unused in a specific term: Let Rec bs0 t' (where bs0 are the
+  complete set of bindings in the let-rec). In the non-recursive case (where
+  let-scoping is linear), we can just check unusedness in the post-term
+  (regardless of its structure, therefore allowing a term where the complete let
+  was removed).
+  *)
+
+  | dc_rec_delete_binding
+      b bs bs' bs'0 t t'
+      (H_pure : pure_binding [] b)
+      (H_unused : unused_in b (Let Rec bs'0 t'))
+      (H_dc_bs : dc_rec bs'0 (Let Rec bs t) (Let Rec bs' t'))
+      : (*-------------------------------------------------*)
+      dc_rec bs'0 (Let Rec (b :: bs) t) (Let Rec bs' t')
+
+  | dc_rec_keep_binding
+      b b' bs bs' bs'0 t t'
+      (H_dc_b : Compat_Binding dc b b')
+      (H_dc_bs : dc_rec bs'0 (Let Rec bs t) (Let Rec bs' t'))
+      : (*-------------------------------------------------*)
+      dc_rec  bs'0 (Let Rec (b :: bs) t) (Let Rec (b' :: bs') t')
+
+  | dc_rec_compat_let_nil_nil
+      t t' bs'0
+      (H_dc_t : dc t t')
+      : (*---------------*)
+      dc_rec bs'0 (Let Rec [] t) (Let Rec [] t')
+.
 
 Scheme dc__ind := Minimality for dc Sort Prop.
 
